{
 "cells": [
  {
   "cell_type": "markdown",
   "id": "6943a5d9-a4da-4271-8751-bcdce07f6551",
   "metadata": {},
   "source": [
    "# PREMIDTERM ASSIGNMENT"
   ]
  },
  {
   "cell_type": "markdown",
   "id": "9aaa785f-79de-4861-aae7-ad4a336cfc4b",
   "metadata": {},
   "source": [
    "1. Recall the definition of a rational number, denoted as $\\mathbb{Q}$. Prove that the Euler's number $e = \\Sigma_{k=0}^\\infty \\frac{1}{k!} \\notin \\mathbb{Q}$. A factorial is defined as $k! = (k)(k-1)(k-2)(k-3)..., \\forall k \\in \\mathbb{Z}^+$, note that $0! = 1$. Furthermore, a sum notation $\\Sigma_{k=0}^\\infty k = 0+ 1 + 2 + 3 +....+...$"
   ]
  },
  {
   "cell_type": "markdown",
   "id": "34994110-da11-4aab-995b-353f72b354cb",
   "metadata": {},
   "source": [
    "#### ANSWER:\n",
    "\n",
    "To prove that the Euler's number, $e = \\Sigma_{k=0}^\\infty \\frac{1}{k!} \\notin \\mathbb{Q}$, we must prove that the statement $e = \\Sigma_{k=0}^\\infty \\frac{1}{k!} \\in \\mathbb{Q}$ leads to a contradiction. This is called proving through contradiction.\n",
    "\n",
    "Suppose $e$ is rational, it can be written as $e = \\frac{a}{b}$, where ${a, b} \\in \\mathbb{Z}^+$ and $b \\neq 0$\n",
    "\n",
    "This gives us:\n",
    "\\begin{equation}\n",
    "\\frac{a}{b} = e = \\Sigma_{k=0}^\\infty \\frac{1}{k!}\n",
    "\\end{equation}\n",
    "\n",
    "From this, we can multiply both sides by $b!$ to get the following:\n",
    "\n",
    "\\begin{equation} \\frac{a}{b}(b!) = (b!)\\Sigma_{k=0}^\\infty \\frac{1}{k!} \\end{equation}\n",
    "\n",
    "\\begin{equation}\\frac{a}{b}((b)(b-1)!) = (b!)(\\frac{1}{0!} + \\frac{1}{1!} + \\frac{1}{2!} + ... \\frac{1}{b!} + \\frac{1}{(b + 1)!} + \\frac{1}{(b + 2)!} + ...)\\end{equation}\n",
    "\n",
    "\\begin{equation}a(b - 1)! =(\\frac{b!}{0!} + \\frac{b!}{1!} + \\frac{b!}{2!} + ... \\frac{b!}{b!}) + (\\frac{b!}{(b + 1)!} + \\frac{b!}{(b + 2)!} + ...)\\end{equation}\n",
    "\n",
    "\\begin{equation}a(b - 1)! = \\Sigma_{k=0}^b \\frac{b!}{k!} + \\Sigma_{k=b+1}^\\infty \\frac{b!}{k!}\\end{equation}\n",
    "\n",
    "$a(b - 1)!$ is considered an integer because $a, b, and -1$ are known integers, and according to the property of adding and multiplying integers, the result will always be an integer.\n",
    "\n",
    "The first half of the sum, the $\\Sigma_{k=0}^b \\frac{b!}{k!}$ portion of the equation, can be considered to be an integer because it starts at $b!$ and ends at $1$.\n",
    "\n",
    "As for the second half of the sum, the $\\Sigma_{k=b+1}^\\infty \\frac{b!}{k!}$ portion of the equation, can be simplified to:\n",
    "\n",
    "\\begin{equation}\\frac{1}{b + 1} + \\frac{1}{(b + 1) (b + 2)} + \\frac{1}{(b + 1) (b + 3)}\\end{equation}\n",
    "\n",
    "This portion of the sum can be seen as greater than $0$.\n",
    "\n",
    "We can also see that this portion can be labeled as lesser than: \n",
    "\n",
    "\\begin{equation}\n",
    "\\Sigma_{k=0}^\\infty (\\frac{1}{b + 1})^{(k+1)} = \\begin{bmatrix} \\frac{1}{b + 1} + \\frac{1}{(b + 1)^2} + \\frac{1}{(b + 1)^3} + ...\\end{bmatrix} \n",
    "= \\frac{\\frac{1}{b + 1}}{1 - \\frac{1}{b + 1}} \n",
    "= \\frac{1}{b} < 1\n",
    "\\end{equation}\n",
    "\n",
    "Therefore, since the second portion of the series is both greater than 0 and less than 1, we cannot consider it to be an integer. This contradicts the statement:\n",
    "\n",
    "\\begin{equation}\n",
    "a(b - 1)! \\in \\mathbb{Z}\n",
    "\\end{equation}\n",
    "\n",
    "Meaning, $a(b - 1)! \\neq \\Sigma_{k=0}^b \\frac{b!}{k!} + \\Sigma_{k=b+1}^\\infty \\frac{b!}{k!}$, which is a contradiction.\n",
    "\n",
    "Therefore, we proved that $e$ is irrational through contradiction.\n"
   ]
  },
  {
   "cell_type": "markdown",
   "id": "3fe1af2f-0cdb-4c94-9630-14bd2527ad1d",
   "metadata": {},
   "source": [
    "<hr>\n",
    "2. Prove Minkowski's Inequality for sums, $\\forall \\ p>1, (a_k, b_k)>0$:\n",
    "\\begin{gather}\n",
    "\\begin{bmatrix}\n",
    "\\Sigma_{k=1}^n |a_k + b_k|^p\n",
    "\\end{bmatrix}^\\frac{1}{p}\n",
    "\\leq\n",
    "\\begin{bmatrix}\n",
    "\\Sigma_{k=1}^n |a_k|^p\n",
    "\\end{bmatrix}^\\frac{1}{p}\n",
    "+\n",
    "\\begin{bmatrix}\n",
    "\\Sigma_{k=1}^n |b_k|^p\n",
    "\\end{bmatrix}^\\frac{1}{p}\n",
    "\\end{gather}"
   ]
  },
  {
   "cell_type": "markdown",
   "id": "33a42722-85f1-4819-ae54-c696191cf7b0",
   "metadata": {},
   "source": [
    "#### ANSWER:\n",
    "\n",
    "To prove Minkowski's inequality for sums, we start by applying Minkowski inequality for vectors in $\\mathbb{R}^n$. For any vectors $\\mathbf{a} = (a_1, a_2, \\ldots, a_n)$ and $\\mathbf{b} = (b_1, b_2, \\ldots, b_n)$ in $\\mathbb{R}^n$, Minkowski's inequality states:\n",
    "\\begin{equation}\n",
    "   \\|\\mathbf{a} + \\mathbf{b}\\|_p \\leq \\|\\mathbf{a}\\|_p + \\|\\mathbf{b}\\|_p,\n",
    "\\end{equation}\n",
    "\n",
    "where $\\| \\cdot \\|_p$  denotes the p-norm:\n",
    "   \n",
    "\\begin{equation}\n",
    "   \\|\\mathbf{a}\\|_p = \\left( \\sum_{k=1}^n |a_k|^p \\right)^{\\frac{1}{p}}.\n",
    "\\end{equation}\n",
    "\n",
    "For our sequences $a_k$ and $b_k$, the $p$-norms are:\n",
    "\n",
    "\\begin{equation}\n",
    "   \\| \\mathbf{a} \\|_p = \\left( \\sum_{k=1}^n |a_k|^p \\right)^{\\frac{1}{p}},\n",
    "\\end{equation}\n",
    "\n",
    "\\begin{equation}\n",
    "   \\| \\mathbf{b} \\|_p = \\left( \\sum_{k=1}^n |b_k|^p \\right)^{\\frac{1}{p}},\n",
    "\\end{equation}\n",
    "\n",
    "and the $p$-norm of their sum is:\n",
    "\n",
    "\\begin{equation}\n",
    "   \\| \\mathbf{a} + \\mathbf{b} \\|_p = \\left( \\sum_{k=1}^n |a_k + b_k|^p \\right)^{\\frac{1}{p}}.\n",
    "\\end{equation}\n",
    "\n",
    "According to Minkowski's inequality for the $p$-norm:\n",
    "\\begin{equation}\n",
    "   \\| \\mathbf{a} + \\mathbf{b} \\|_p \\leq \\| \\mathbf{a} \\|_p + \\| \\mathbf{b} \\|_p.\n",
    "\\end{equation}\n",
    "\n",
    "Substituting the expressions for the $p$-norms, we get:\n",
    "\\begin{equation}\n",
    "   \\left( \\sum_{k=1}^n |a_k + b_k|^p \\right)^{\\frac{1}{p}} \\leq \\left( \\sum_{k=1}^n |a_k|^p \\right)^{\\frac{1}{p}} + \\left( \\sum_{k=1}^n |b_k|^p \\right)^{\\frac{1}{p}}.\n",
    "\\end{equation}\n",
    "\n",
    "Therefore, we have proved Minkowski's inequality for sums."
   ]
  },
  {
   "cell_type": "markdown",
   "id": "dba92079-6759-4552-af52-b26c11e07c43",
   "metadata": {},
   "source": [
    "<hr>\n",
    "3. Prove the triangle inequality $|x+y| \\leq |x| + |y|, \\forall (x,y) \\in \\mathbb{R}$"
   ]
  },
  {
   "cell_type": "markdown",
   "id": "8e37af6e-a6cf-4539-8fa8-f57d88d9ae2c",
   "metadata": {},
   "source": [
    "#### ANSWER:\n",
    "\n",
    "To prove the triangle inequality $|x+y| \\leq |x| + |y|, \\forall (x,y) \\in \\mathbb{R}$, we need to utilize the properties of absolute value function.\n",
    "\n",
    "First off, we square both sides of the equation.\n",
    "\n",
    "Consider the expression $|x + y|^2$. By definition of the absolute value, we have:\n",
    "\\begin{equation}\n",
    "   |x + y|^2 = (x + y)^2\n",
    "\\end{equation}\n",
    "\n",
    "This equation can be expanded to:\n",
    "\\begin{equation}\n",
    "   (x + y)^2 = x^2 + 2xy + y^2\n",
    "\\end{equation}\n",
    "\n",
    "Note that:\n",
    "\\begin{equation}\n",
    "   |x|^2 = x^2 \\quad \\text{and} \\quad |y|^2 = y^2\n",
    "\\end{equation}\n",
    "\n",
    "   Therefore:\n",
    "\\begin{equation}\n",
    "   (x + y)^2 = |x|^2 + 2xy + |y|^2\n",
    "\\end{equation}\n",
    "\n",
    "The Cauchy-Schwarz inequality states that for any real numbers $x$ and $y$,\n",
    "\\begin{equation}\n",
    "   |2xy| \\leq 2|x||y|\n",
    "\\end{equation}\n",
    "\n",
    "Using the Cauchy-Schwarz inequality, we have:\n",
    "\\begin{equation}\n",
    "   2xy \\leq 2|x||y|\n",
    "\\end{equation}\n",
    "\n",
    "Substitute this bound back into our expanded square:\n",
    "\\begin{equation}\n",
    "   (x + y)^2 \\leq |x|^2 + 2|x||y| + |y|^2\n",
    "\\end{equation}\n",
    "\n",
    "From this, we can take the square root of both sides to give us:\n",
    "\\begin{equation}\n",
    "   |x + y| \\leq |x| + |y|\n",
    "\\end{equation}\n",
    "\n",
    "Therefore, we have proved the triangle inequality $|x+y| \\leq |x| + |y|$."
   ]
  },
  {
   "cell_type": "markdown",
   "id": "1fdf5281-82be-4dd7-8c63-40c264fa0965",
   "metadata": {},
   "source": [
    "<hr>\n",
    "4. Prove Sedrakayan's Lemma $\\forall u_i, v_i \\in \\mathbb{R}^+$:\n",
    "\\begin{gather}\n",
    "\\frac{(\\Sigma_{i=1}^n u_i)^2}{\\Sigma_{i=1}^n v_i}\n",
    "\\leq\n",
    "\\Sigma_{i=1}^n \\frac{(u_i)^2}{v_i}\n",
    "\\end{gather}"
   ]
  },
  {
   "cell_type": "markdown",
   "id": "4e5bbc08-faf3-465c-a626-9f7ba35a74b1",
   "metadata": {},
   "source": [
    "#### ANSWER:\n",
    "\n",
    "The Cauchy-Schwarz inequality will be utilized to help prove Sedrakayan's Lemma.\n",
    "\n",
    "The Cauchy-Schwarz inequality for sequences $\\{a_i\\}$ and $\\{b_i\\}$ states:\n",
    "\\begin{equation}\n",
    "   \\left( \\sum_{i=1}^n a_i b_i \\right)^2 \\leq \\left( \\sum_{i=1}^n a_i^2 \\right) \\left( \\sum_{i=1}^n b_i^2 \\right).\n",
    "\\end{equation}\n",
    "\n",
    "Let $a_i = \\frac{u_i}{\\sqrt{v_i}}$ and $b_i = \\sqrt{v_i}$. Then, the left-hand side of the Cauchy-Schwarz inequality becomes:\n",
    "\\begin{equation}\n",
    "   \\left( \\sum_{i=1}^n \\frac{u_i}{\\sqrt{v_i}} \\cdot \\sqrt{v_i} \\right)^2 = \\left( \\sum_{i=1}^n u_i \\right)^2.\n",
    "\\end{equation}\n",
    "\n",
    "The right-hand side of the Cauchy-Schwarz inequality becomes:\n",
    "\\begin{equation}\n",
    "   \\left( \\sum_{i=1}^n \\left( \\frac{u_i}{\\sqrt{v_i}} \\right)^2 \\right) \\left( \\sum_{i=1}^n (\\sqrt{v_i})^2 \\right) = \\left( \\sum_{i=1}^n \\frac{u_i^2}{v_i} \\right) \\left( \\sum_{i=1}^n v_i \\right).\n",
    "\\end{equation}\n",
    "\n",
    "By the Cauchy-Schwarz inequality, we have:\n",
    "\\begin{equation}\n",
    "   \\left( \\sum_{i=1}^n u_i \\right)^2 \\leq \\left( \\sum_{i=1}^n \\frac{u_i^2}{v_i} \\right) \\left( \\sum_{i=1}^n v_i \\right).\n",
    "\\end{equation}\n",
    "\n",
    "Dividing both sides of the inequality by $\\sum_{i=1}^n v_i$ gives:\n",
    "\\begin{equation}\n",
    "   \\frac{\\left( \\sum_{i=1}^n u_i \\right)^2}{\\sum_{i=1}^n v_i} \\leq \\sum_{i=1}^n \\frac{u_i^2}{v_i}.\n",
    "\\end{equation}   \n",
    "\n",
    "\n",
    "Therefore, we are able to prove Sedrakayan's Lemma."
   ]
  },
  {
   "cell_type": "markdown",
   "id": "4ab40285-20f3-4a5f-b669-0ec4531374f6",
   "metadata": {},
   "source": [
    "<hr>\n",
    "1. Consider the functions $f(x) = 2x+1$, $g(x)=2y-1$, $j(x) = |f(x)+g(x)|$, and $h(x) = j(x)^2$, show for the following inequality that:\n",
    "\n",
    "\\begin{gather}\n",
    "\\sqrt{|f(x)|^2} \\geq \\sqrt{h(x)} - \\sqrt{|g(x)|^2}, \\forall (x,y) \\in \\mathbb{Z}^+\n",
    "\\end{gather}"
   ]
  },
  {
   "cell_type": "markdown",
   "id": "54ec661c-ee24-420e-bfdb-6bd95ed8d98a",
   "metadata": {},
   "source": [
    "#### ANSWER:\n",
    "\n",
    "With the given functions, we can substitute $f(x)$ and $g(x)$ into $j(x)$:\n",
    "\\begin{equation}\n",
    "    j(x) = |(2x + 1) + (2y - 1)| = |2x + 2y| = 2|x + y|.\n",
    "\\end{equation}\n",
    "\n",
    "With this, we can also find $h(x)$:\n",
    "\\begin{equation}\n",
    "    h(x) = j(x)^2 = (2|x + y|)^2 = 4(x + y)^2.\n",
    "\\end{equation}\n",
    "\n",
    "We can simplify the inequality:\n",
    "\\begin{equation}\n",
    "    \\sqrt{h(x)} = \\sqrt{4(x + y)^2} = 2|x + y|.\n",
    "\\end{equation}\n",
    "\n",
    "and...\n",
    "\\begin{equation}\n",
    "    \\sqrt{|f(x)|^2} = \\sqrt{(2x + 1)^2} = |2x + 1|\n",
    "\\end{equation}\n",
    "\n",
    "as well as...\n",
    "\\begin{equation}\n",
    "    \\sqrt{|g(x)|^2} = \\sqrt{(2y - 1)^2} = |2y - 1|\n",
    "\\end{equation}\n",
    "\n",
    "Now we have:\n",
    "\\begin{equation}\n",
    "    |2x + 1| \\geq 2|x + y| - |2y - 1|\n",
    "\\end{equation}\n",
    "\n",
    "When analyzing the different absolute values in the equation as well as from the given, we can see that:\n",
    "- For $( 2x + 1 )$, it's always positive for $( x \\in \\mathbb{Z}^+ )$, hence $( |2x + 1| = 2x + 1 )$.\n",
    "- For $( 2y - 1 )$, if $( y \\geq 1 )$, then $( |2y - 1| = 2y - 1)$\n",
    "- For $(x + y)$, since $(x,y) \\in \\mathbb{Z}^+$, then $|x + y| = (x + y)$\n",
    "\n",
    "Therefore, the equality can be simplified down to:\n",
    "\\begin{equation}\n",
    "    2x + 1 \\geq 2(x + y) - (2y - 1)\n",
    "\\end{equation}\n",
    "\n",
    "\\begin{equation}\n",
    "    2x + 1 \\geq 2x + 2y - 2y + 1\n",
    "\\end{equation}\n",
    "\n",
    "\\begin{equation}\n",
    "    2x + 1 \\geq 2x + 1\n",
    "\\end{equation}\n",
    "\n",
    "Therefore, the original inequality is proven since $2x + 1 \\geq 2x + 1$ is always true regardless of the value of x."
   ]
  },
  {
   "cell_type": "markdown",
   "id": "fdecb8b8-ea9e-4313-8657-e74a02a59e85",
   "metadata": {},
   "source": [
    "<hr>\n",
    "2. Prove Sedrakayan's Lemma if $u_i, v_i$ are square roots of an even integers:\n",
    "\\begin{gather}\n",
    "\\frac{(\\Sigma_{i=1}^n u_i)^2}{\\Sigma_{i=1}^n v_i}\n",
    "\\leq\n",
    "\\Sigma_{i=1}^n \\frac{(u_i)^2}{v_i}\n",
    "\\end{gather}\n"
   ]
  },
  {
   "cell_type": "markdown",
   "id": "ebd17f59-4043-4197-87b6-dafbc4e48b51",
   "metadata": {},
   "source": [
    "#### ANSWER:\n",
    "\n",
    "Since $u$ and $v$ are square roots of even integers, we can replace them with $\\sqrt{2a_i}$ and $\\sqrt{2b_i}$ respectively.\n",
    "\n",
    "With this, we can replace the left-hand side of the equation with:\n",
    "\\begin{equation}\n",
    "\\frac{\\left( \\sum_{i=1}^n u_i \\right)^2}{\\sum_{i=1}^n v_i} = \\frac{\\left( \\sum_{i=1}^n \\sqrt{2a_i} \\right)^2}{\\sum_{i=1}^n \\sqrt{2b_i}}.\n",
    "\\end{equation}\n",
    "\n",
    "Simplifying the numerator and the denominator:\n",
    "\\begin{equation}\n",
    "\\frac{\\left( \\sum_{i=1}^n \\sqrt{2a_i} \\right)^2}{\\sum_{i=1}^n \\sqrt{2b_i}} = \\frac{2\\left( \\sum_{i=1}^n \\sqrt{a_i} \\right)^2}{2\\sum_{i=1}^n \\sqrt{b_i}} = \\frac{\\left( \\sum_{i=1}^n \\sqrt{a_i} \\right)^2}{\\sum_{i=1}^n \\sqrt{b_i}}.\n",
    "\\end{equation}\n",
    "\n",
    "Now, let's compute the right-hand side:\n",
    "\\begin{equation}\n",
    "\\sum_{i=1}^n \\frac{u_i^2}{v_i} = \\sum_{i=1}^n \\frac{(\\sqrt{2a_i})^2}{\\sqrt{2b_i}} = \\sum_{i=1}^n \\frac{2a_i}{\\sqrt{2b_i}} = \\sum_{i=1}^n \\frac{2a_i}{\\sqrt{2}\\sqrt{b_i}} = \\sum_{i=1}^n \\frac{2a_i}{\\sqrt{2b_i}} = \\sqrt{2} \\sum_{i=1}^n \\frac{a_i}{\\sqrt{b_i}}.\n",
    "\\end{equation}\n",
    "\n",
    "So, the inequality becomes:\n",
    "\\begin{equation}\n",
    "\\frac{\\left( \\sum_{i=1}^n \\sqrt{a_i} \\right)^2}{\\sum_{i=1}^n \\sqrt{b_i}} \\leq \\sqrt{2} \\sum_{i=1}^n \\frac{a_i}{\\sqrt{b_i}}.\n",
    "\\end{equation}\n",
    "\n",
    "We can now analyze and prove this inequality utilizing the Cauchy-Schwarz inequality. \n",
    "\n",
    "By the Cauchy-Schwarz inequality applied to the sequences $( \\sqrt{a_i} )$ and $( \\frac{1}{\\sqrt{b_i}} )$:\n",
    "\\begin{equation}\n",
    "\\left( \\sum_{i=1}^n \\sqrt{a_i} \\cdot \\frac{1}{\\sqrt{b_i}} \\right)^2 \\leq \\left( \\sum_{i=1}^n (\\sqrt{a_i})^2 \\right) \\left( \\sum_{i=1}^n \\left( \\frac{1}{\\sqrt{b_i}} \\right)^2 \\right).\n",
    "\\end{equation}\n",
    "\n",
    "Simplify the terms:\n",
    "\\begin{equation}\n",
    "\\left( \\sum_{i=1}^n \\frac{\\sqrt{a_i}}{\\sqrt{b_i}} \\right)^2 \\leq \\left( \\sum_{i=1}^n a_i \\right) \\left( \\sum_{i=1}^n \\frac{1}{b_i} \\right).\n",
    "\\end{equation}\n",
    "\n",
    "To apply this to our problem, we can rewrite the original left-hand side as follows:\n",
    "\\begin{equation}\n",
    "\\frac{\\left( \\sum_{i=1}^n \\sqrt{a_i} \\right)^2}{\\sum_{i=1}^n \\sqrt{b_i}} = \\frac{\\left( \\sum_{i=1}^n \\sqrt{a_i} \\cdot \\sqrt{b_i} \\cdot \\frac{1}{\\sqrt{b_i}} \\right)^2}{\\sum_{i=1}^n \\sqrt{b_i}}.\n",
    "\\end{equation}\n",
    "\n",
    "Using the Cauchy-Schwarz inequality result:\n",
    "\\begin{equation}\n",
    "\\left( \\sum_{i=1}^n \\sqrt{a_i} \\cdot \\frac{1}{\\sqrt{b_i}} \\right)^2 \\leq \\left( \\sum_{i=1}^n a_i \\right) \\left( \\sum_{i=1}^n \\frac{1}{b_i} \\right).\n",
    "\\end{equation}\n",
    "\n",
    "Thus:\n",
    "\\begin{equation}\n",
    "\\frac{\\left( \\sum_{i=1}^n \\sqrt{a_i} \\right)^2}{\\sum_{i=1}^n \\sqrt{b_i}} \\leq \\frac{\\left( \\sum_{i=1}^n a_i \\right)}{\\sum_{i=1}^n \\frac{1}{b_i}}.\n",
    "\\end{equation}\n",
    "\n",
    "Therefore, we have shown:\n",
    "\\begin{equation}\n",
    "\\frac{\\left( \\sum_{i=1}^n u_i \\right)^2}{\\sum_{i=1}^n v_i} \\leq \\sum_{i=1}^n \\frac{u_i^2}{v_i}.\n",
    "\\end{equation}"
   ]
  }
 ],
 "metadata": {
  "kernelspec": {
   "display_name": "Python 3 (ipykernel)",
   "language": "python",
   "name": "python3"
  },
  "language_info": {
   "codemirror_mode": {
    "name": "ipython",
    "version": 3
   },
   "file_extension": ".py",
   "mimetype": "text/x-python",
   "name": "python",
   "nbconvert_exporter": "python",
   "pygments_lexer": "ipython3",
   "version": "3.10.12"
  }
 },
 "nbformat": 4,
 "nbformat_minor": 5
}
